PREFIX : <https://linked.data.gov.au/def/geocode-types/>
PREFIX astatus: <https://linked.data.gov.au/def/reg-statuses/>
PREFIX cs: <https://linked.data.gov.au/def/geocode-types>
PREFIX droles: <https://linked.data.gov.au/def/data-roles/>
PREFIX owl: <http://www.w3.org/2002/07/owl#>
PREFIX prov: <http://www.w3.org/ns/prov#>
PREFIX rdfs: <http://www.w3.org/2000/01/rdf-schema#>
PREFIX reg: <http://purl.org/linked-data/registry#>
PREFIX schema: <https://schema.org/>
PREFIX skos: <http://www.w3.org/2004/02/skos/core#>
PREFIX unggim: <https://linked.data.gov.au/def/unggim-themes/>
PREFIX xsd: <http://www.w3.org/2001/XMLSchema#>

<https://linked.data.gov.au/def/location-addressing/DTSpecCode> a rdfs:Datatype ;
    sdo:name "Queensland Location Addresses Data Transfer Specification Code" ;
    sdo:description "The datatype code to use for the address data exchange system as seen in the Queensland Location Addresses Data Transfer Specification" ;
.

:building-access-point
    a skos:Concept ;
    rdfs:isDefinedBy cs: ;
    skos:altLabel "BAP"@en ;
    skos:definition "Point of access to the building. "@en ;
    skos:historyNote "AS 4590.1:2017 (Standards Australia). " ;
    skos:inScheme cs: ;
    skos:notation "BAP"^^<https://linked.data.gov.au/def/location-addressing/DTSpecCode> ;
    skos:prefLabel "Building Access Point"@en ;
    skos:topConceptOf cs: ;
.

:building-centroid
    a skos:Concept ;
    rdfs:isDefinedBy cs: ;
    skos:altLabel "BC"@en ;
    skos:definition "Point as centre of building and lying within its bounds (e.g. for u-shaped building). "@en ;
    skos:historyNote "AS 4590.1:2017 (Standards Australia). " ;
    skos:inScheme cs: ;
    skos:notation "BC"^^<https://linked.data.gov.au/def/location-addressing/DTSpecCode> ;
    skos:prefLabel "Building Centroid"@en ;
    skos:topConceptOf cs: ;
.

:centreline-dropped-driveway-frontage
    a skos:Concept ;
    rdfs:isDefinedBy cs: ;
    skos:altLabel "CDDF"@en ;
    skos:definition "A point on the road centre-line opposite the centre of the driveway access to an address site. "@en ;
    skos:historyNote "Added by Queensland 2024-06-12. " ;
    skos:inScheme cs: ;
    skos:prefLabel "Centreline Dropped Driveway Frontage"@en ;
.

:centreline-dropped-frontage
    a skos:Concept ;
    rdfs:isDefinedBy cs: ;
    skos:altLabel "CDF"@en ;
    skos:definition "A point on the road centre-line opposite the centre of the road frontage of an address site. "@en ;
    skos:historyNote "AS 4590.1:2017 (Standards Australia). " ;
    skos:inScheme cs: ;
    skos:notation "CDF"^^<https://linked.data.gov.au/def/location-addressing/DTSpecCode> ;
    skos:prefLabel "Centreline Dropped Frontage"@en ;
    skos:topConceptOf cs: ;
.

:electricity-connection-point
    a skos:Concept ;
    rdfs:isDefinedBy cs: ;
    skos:altLabel "ECP"@en ;
    skos:definition "Electricity connection point (e.g. box, or underground chamber). "@en ;
    skos:historyNote "Geocoded National Address File (G-NAF) data definitions. " ;
    skos:inScheme cs: ;
    skos:prefLabel "Electricity Connection Point"@en ;
.

:electricity-meter
    a skos:Concept ;
    rdfs:isDefinedBy cs: ;
    skos:altLabel "EM"@en ;
    skos:definition "Electricity meter point (e.g. box, or underground chamber). "@en ;
    skos:historyNote "Geocoded National Address File (G-NAF) data definitions. " ;
    skos:inScheme cs: ;
    skos:prefLabel "Electricity Meter"@en ;
.

:emergency-access
    a skos:Concept ;
    rdfs:isDefinedBy cs: ;
    skos:altLabel "EA"@en ;
    skos:definition "Specific building or address site access point for emergency services. "@en ;
    skos:historyNote "AS 4590.1:2017 (Standards Australia). " ;
    skos:inScheme cs: ;
    skos:notation "EA"^^<https://linked.data.gov.au/def/location-addressing/DTSpecCode> ;
    skos:prefLabel "Emergency Access"@en ;
    skos:topConceptOf cs: ;
.

:emergency-access-secondary
    a skos:Concept ;
    rdfs:isDefinedBy cs: ;
    skos:altLabel "EAS"@en ;
    skos:definition "Specific building or address site secondary access point for emergency services. "@en ;
    skos:historyNote "AS 4590.1:2017 (Standards Australia). " ;
    skos:inScheme cs: ;
    skos:notation "EAS"^^<https://linked.data.gov.au/def/location-addressing/DTSpecCode> ;
    skos:prefLabel "Emergency Access Secondary"@en ;
    skos:topConceptOf cs: ;
.

:front-door-access
    a skos:Concept ;
    rdfs:isDefinedBy cs: ;
    skos:altLabel "FDA"@en ;
    skos:definition "Front door of building"@en ;
    skos:historyNote "AS 4590.1:2017 (Standards Australia). " ;
    skos:inScheme cs: ;
    skos:notation "FDA"^^<https://linked.data.gov.au/def/location-addressing/DTSpecCode> ;
    skos:prefLabel "Front Door Access"@en ;
    skos:topConceptOf cs: ;
.

:frontage-centre
    a skos:Concept ;
    rdfs:isDefinedBy cs: ;
    skos:altLabel "FC"@en ;
    skos:definition "Point on the centre of the address site frontage. "@en ;
    skos:historyNote "AS 4590.1:2017 (Standards Australia). " ;
    skos:inScheme cs: ;
    skos:notation "FC"^^<https://linked.data.gov.au/def/location-addressing/DTSpecCode> ;
    skos:prefLabel "Frontage Centre"@en ;
    skos:topConceptOf cs: ;
.

:frontage-centre-setback
    a skos:Concept ;
    rdfs:isDefinedBy cs: ;
    skos:altLabel "FCS"@en ;
    skos:definition "A point set back from the centre of the road frontage within an address site. "@en ;
    skos:historyNote "AS 4590.1:2017 (Standards Australia). " ;
    skos:inScheme cs: ;
    skos:notation "FCS"^^<https://linked.data.gov.au/def/location-addressing/DTSpecCode> ;
    skos:prefLabel "Frontage Centre Setback"@en ;
    skos:topConceptOf cs: ;
.

:gas-connection-point
    a skos:Concept ;
    rdfs:isDefinedBy cs: ;
    skos:altLabel "GCP"@en ;
    skos:definition "Gas connection point (e.g. box, or underground chamber). "@en ;
    skos:historyNote "Geocoded National Address File (G-NAF) data definitions. " ;
    skos:inScheme cs: ;
    skos:prefLabel "Gas Connection Point"@en ;
.

:gas-meter
    a skos:Concept ;
    rdfs:isDefinedBy cs: ;
    skos:altLabel "GM"@en ;
    skos:definition "Gas meter point (e.g. box, or underground chamber). "@en ;
    skos:historyNote "Geocoded National Address File (G-NAF) data definitions. " ;
    skos:inScheme cs: ;
    skos:prefLabel "Gas Meter"@en ;
.

:internet-connection-point
    a skos:Concept ;
    rdfs:isDefinedBy cs: ;
    skos:altLabel "ICP"@en ;
    skos:definition "Internet connection point (e.g. box, or underground chamber). "@en ;
    skos:historyNote "Geocoded National Address File (G-NAF) data definitions. " ;
    skos:inScheme cs: ;
    skos:prefLabel "Internet Connection Point"@en ;
.

:letterbox
    a skos:Concept ;
    rdfs:isDefinedBy cs: ;
    skos:altLabel "LB"@en ;
    skos:definition "Place where mail is deposited. "@en ;
    skos:historyNote "AS 4590.1:2017 (Standards Australia). " ;
    skos:inScheme cs: ;
    skos:notation "LB"^^<https://linked.data.gov.au/def/location-addressing/DTSpecCode> ;
    skos:prefLabel "Letterbox"@en ;
    skos:topConceptOf cs: ;
.

:property-access-aeroplane
    a skos:Concept ;
    rdfs:isDefinedBy cs: ;
    skos:altLabel "PAPA"@en ;
    skos:definition "Access point by aeroplane to an address site, such as an airstrip. "@en ;
    skos:historyNote "Added by Queensland 2024-06-12. " ;
    skos:inScheme cs: ;
    skos:prefLabel "Property Access Aeroplane"@en ;
.

:property-access-helicopter
    a skos:Concept ;
    rdfs:isDefinedBy cs: ;
    skos:altLabel "PAPH"@en ;
    skos:definition "Access point by helicopter to an address site, such as a helipad. "@en ;
    skos:historyNote "Added by Queensland 2024-06-12. " ;
    skos:inScheme cs: ;
    skos:prefLabel "Property Access Helicopter"@en ;
.

:property-access-point
    a skos:Concept ;
    rdfs:isDefinedBy cs: ;
    skos:altLabel "PAP"@en ;
    skos:definition "Access point to the address site. "@en ;
    skos:historyNote "AS 4590.1:2017 (Standards Australia) with definition amended for clarity 2024-06-11. " ;
    skos:inScheme cs: ;
    skos:notation "PAP"^^<https://linked.data.gov.au/def/location-addressing/DTSpecCode> ;
    skos:narrower
        :centreline-dropped-driveway-frontage ,
        :driveway-frontage ,
        :property-access-aeroplane ,
        :property-access-helicopter ,
        :property-access-point-setback ,
        :property-access-water ;
    skos:prefLabel "Property Access Point"@en ;
    skos:topConceptOf cs: ;
.

:property-access-water
    a skos:Concept ;
    rdfs:isDefinedBy cs: ;
    skos:altLabel "PAPW"@en ;
    skos:definition "Access point from a water feature to an address site. "@en ;
    skos:historyNote "Added by Queensland 2024-06-12. " ;
    skos:inScheme cs: ;
    skos:prefLabel "Property Access Water"@en ;
.

:property-centroid
    a skos:Concept ;
    rdfs:isDefinedBy cs: ;
    skos:altLabel "PC"@en ;
    skos:definition "Point of centre of parcels making up an address site and lying within its boundaries (e.g. for l-shaped address site). "@en ;
    skos:historyNote "AS 4590.1:2017 (Standards Australia). " ;
    skos:inScheme cs: ;
    skos:notation "PC"^^<https://linked.data.gov.au/def/location-addressing/DTSpecCode> ;
    skos:prefLabel "Property Centroid"@en ;
    skos:topConceptOf cs: ;
.

:service-connection-point
    a skos:Concept ;
    rdfs:isDefinedBy cs: ;
    skos:altLabel "SCP"@en ;
    skos:definition "The utility connection point (e.g. box, or underground chamber). "@en ;
    skos:historyNote "AS 4590.1:2017 (Standards Australia). " ;
    skos:inScheme cs: ;
    skos:notation "STCP"^^<https://linked.data.gov.au/def/location-addressing/DTSpecCode> ;
    skos:narrower
        :electricity-connection-point ,
        :gas-connection-point ,
        :internet-connection-point ,
        :sewerage-connection-point ,
        :telephone-connection-point ,
        :water-connection-point ;
    skos:prefLabel "Service Connection Point"@en ;
    skos:topConceptOf cs: ;
.

:service-meter
    a skos:Concept ;
    rdfs:isDefinedBy cs: ;
    skos:altLabel "SM"@en ;
    skos:definition "The utility meter (e.g. box, or underground chamber). "@en ;
    skos:historyNote "AS 4590.1:2017 (Standards Australia). " ;
    skos:inScheme cs: ;
    skos:notation "STM"^^<https://linked.data.gov.au/def/location-addressing/DTSpecCode> ;
    skos:narrower
        :electricity-meter ,
        :gas-meter ,
        :water-meter ;
    skos:prefLabel "Service Meter"@en ;
    skos:topConceptOf cs: ;
.

:sewerage-connection-point
    a skos:Concept ;
    rdfs:isDefinedBy cs: ;
    skos:altLabel "SCP"@en ;
    skos:definition "Sewerage connection point (e.g. box, or underground chamber). "@en ;
    skos:historyNote "Geocoded National Address File (G-NAF) data definitions. " ;
    skos:inScheme cs: ;
    skos:prefLabel "Sewerage Connection Point"@en ;
.

:telephone-connection-point
    a skos:Concept ;
    rdfs:isDefinedBy cs: ;
    skos:altLabel "TCP"@en ;
    skos:definition "Telephone connection point (e.g. box, or underground chamber). "@en ;
    skos:historyNote "Geocoded National Address File (G-NAF) data definitions. " ;
    skos:inScheme cs: ;
    skos:prefLabel "Telephone Connection Point"@en ;
.

:unit-centroid
    a skos:Concept ;
    rdfs:isDefinedBy cs: ;
    skos:altLabel "UC"@en ;
    skos:definition "Point at centre of unit and lying within its bounds (e.g. for u-shaped unit). "@en ;
    skos:historyNote "AS 4590.1:2017 (Standards Australia). " ;
    skos:inScheme cs: ;
    skos:notation "UC"^^<https://linked.data.gov.au/def/location-addressing/DTSpecCode> ;
    skos:prefLabel "Unit Centroid"@en ;
    skos:topConceptOf cs: ;
.

:water-connection-point
    a skos:Concept ;
    rdfs:isDefinedBy cs: ;
    skos:altLabel "WCP"@en ;
    skos:definition "Water connection point (e.g. box, or underground chamber). "@en ;
    skos:historyNote "Geocoded National Address File (G-NAF) data definitions. " ;
    skos:inScheme cs: ;
    skos:prefLabel "Water Connection Point"@en ;
.

:water-meter
    a skos:Concept ;
    rdfs:isDefinedBy cs: ;
    skos:altLabel "WM"@en ;
    skos:definition "Water meter point (e.g. box, or underground chamber). "@en ;
    skos:historyNote "Geocoded National Address File (G-NAF) data definitions. " ;
    skos:inScheme cs: ;
    skos:prefLabel "Water Meter"@en ;
.

<https://linked.data.gov.au/org/qsi>
    a schema:Organization ;
    schema:name "Queensland Spatial Information" ;
    schema:url "https://www.resources.qld.gov.au/data-mapping"^^xsd:anyURI ;
.

:driveway-frontage
    a skos:Concept ;
    rdfs:isDefinedBy cs: ;
    skos:altLabel "DF"@en ;
    skos:definition "Centre of driveway on address site frontage; access point from a road to an address site. "@en ;
    skos:historyNote "AS 4590.1:2017 (Standards Australia) with definition amended for clarity 2024-06-11. " ;
    skos:inScheme cs: ;
    skos:notation "DF"^^<https://linked.data.gov.au/def/location-addressing/DTSpecCode> ;
    skos:prefLabel "Driveway Frontage"@en ;
.

:property-access-point-setback
    a skos:Concept ;
    rdfs:isDefinedBy cs: ;
    skos:altLabel "PAPS"@en ;
    skos:definition "Point set back from the access point to an address site. "@en ;
    skos:historyNote "AS 4590.1:2017 (Standards Australia) with definition amended for clarity 2024-06-11. " ;
    skos:inScheme cs: ;
    skos:notation "PAPS"^^<https://linked.data.gov.au/def/location-addressing/DTSpecCode> ;
    skos:prefLabel "Property Access Point Setback"@en ;
.

<https://linked.data.gov.au/org/icsm>
    a schema:Organization ;
    schema:name "Intergovernmental Committee on Surveying & Mapping" ;
    schema:url "https://icsm.gov.au"^^xsd:anyURI ;
.

cs:
    a skos:ConceptScheme ;
    reg:status astatus:experimental ;
    owl:versionIRI :1.0 ;
    owl:versionInfo "1.0" ;
    skos:definition "This vocabulary describes types of geocode. A geocode is a point location with a specialised type or a role which can be assigned to position something. "@en ;
    skos:hasTopConcept
        :building-access-point ,
        :building-centroid ,
        :centreline-dropped-frontage ,
        :driveway-frontage ,
        :emergency-access ,
        :emergency-access-secondary ,
        :front-door-access ,
        :frontage-centre ,
        :frontage-centre-setback ,
        :letterbox ,
        :property-access-point ,
        :property-access-point-setback ,
        :property-centroid ,
        :service-connection-point ,
        :service-meter ,
        :unit-centroid ;
    skos:historyNote "This vocabulary contains geocodes types in common usage at the time of publishing. These are sourced from standards including AS4590.1:2017 and the Queensland and Geocoded National Address File (G-NAF) data definitions.  address datasets." ;
    skos:prefLabel "Geocode Types"@en ;
    prov:qualifiedAttribution
        [
            prov:agent <https://linked.data.gov.au/org/icsm> ;
            prov:hadRole droles:custodian ;
        ] ;
    schema:creator <https://linked.data.gov.au/org/qsi> ;
    schema:dateCreated "2023-05-11"^^xsd:date ;
    schema:dateModified "2023-11-30"^^xsd:date ;
    schema:identifier "geocode-types"^^xsd:token ;
    schema:keywords unggim:Addresses ;
    schema:publisher <https://linked.data.gov.au/org/icsm> ;
.
